lib/hst/Hacl.Cast.fst
@@ -1,17 +1,28 @@
 module Hacl.Cast
 
-module U8  = Hacl.UInt8
-module U32 = Hacl.UInt32
-module U64 = Hacl.UInt64
+module S8  = Hacl.UInt8
+module S32 = Hacl.UInt32
+module S64 = Hacl.UInt64
+module U32 = FStar.UInt32
 
-let op_At_Percent = FStar.Int.op_At_Percent
+(** Uints to Sints **)
+assume val sint8_to_sint64: a:S8.t -> Tot (b:S64.t{S64.v b = S8.v a})
+assume val sint8_to_sint32: a:S8.t -> Tot (b:S32.t{S32.v b = S8.v a})
 
-(** Uints to Uints **)
-assume val uint8_to_uint64: a:U8.t -> Tot (b:U64.t{U64.v b = U8.v a})
-assume val uint8_to_uint32: a:U8.t -> Tot (b:U32.t{U32.v b = U8.v a})
+assume val sint32_to_sint64: a:S32.t -> Tot (b:S64.t{S64.v b = S32.v a})
+assume val sint32_to_sint8 : a:S32.t -> Tot (b:S8.t{S8.v b = S32.v a % pow2 8})
 
-assume val uint32_to_uint64: a:U32.t -> Tot (b:U64.t{U64.v b = U32.v a})
-assume val uint32_to_uint8 : a:U32.t -> Tot (b:U8.t{U8.v b = U32.v a % pow2 8})
+assume val sint64_to_sint32: a:S64.t -> Tot (b:S32.t{S32.v b = S64.v a % pow2 32})
+assume val sint64_to_sint8 : a:S64.t -> Tot (b:S8.t{S8.v b = S64.v a % pow2 8})
 
-assume val uint64_to_uint32: a:U64.t -> Tot (b:U32.t{U32.v b = U64.v a % pow2 32})
-assume val uint64_to_uint8 : a:U64.t -> Tot (b:U8.t{U8.v b = U64.v a % pow2 8})
+assume val uint64_to_sint64: a:UInt64.t -> Tot (b:S64.t{S64.v b = UInt64.v a})
+assume val uint64_to_sint32: a:UInt64.t -> Tot (b:S32.t{S32.v b = UInt64.v a % pow2 32})
+assume val uint64_to_sint8: a:UInt64.t -> Tot (b:S8.t{S8.v b = UInt64.v a % pow2 8})
+
+assume val uint32_to_sint64: a:UInt32.t -> Tot (b:S64.t{S64.v b = UInt32.v a})
+assume val uint32_to_sint32: a:UInt32.t -> Tot (b:S32.t{S32.v b = UInt32.v a % pow2 32})
+assume val uint32_to_sint8: a:UInt32.t -> Tot (b:S8.t{S8.v b = UInt32.v a % pow2 8})
+
+assume val uint8_to_sint64: a:UInt8.t -> Tot (b:S64.t{S64.v b = UInt8.v a})
+assume val uint8_to_sint32: a:UInt8.t -> Tot (b:S32.t{S32.v b = UInt8.v a % pow2 32})
+assume val uint8_to_sint8: a:UInt8.t -> Tot (b:S8.t{S8.v b = UInt8.v a % pow2 8})
